Challenge/Blake2f/ProofSupport.lean
@@ -1,5 +1,6 @@
 import Challenge.Blake2f.ProofSupport.Bytecode
 import Challenge.Blake2f.ProofSupport.Algorithm
+import Challenge.Blake2f.ProofSupport.Input
 import Challenge.Blake2f.ProofSupport.InitialState
 import Challenge.Blake2f.ProofSupport.Memory
 import Challenge.Blake2f.ProofSupport.Word
